src/formal-semantics/lean/PyCSL/SOS.lean
@@ -169,9 +169,9 @@ inductive Exec : ExecState → Stmt → Outcome → Prop where
     Exec es (.threadEntry body) out
 
   | execFor (es : ExecState) (x arr : Ident) (inv var : ContractExpr)
-      (body : Stmt) (out : Outcome) :
-    Exec es (desugar (.for_ x arr inv var body)) out →
-    Exec es (.for_ x arr inv var body) out
+      (body : Stmt) (aim : Bool) (out : Outcome) :
+    Exec es (desugar (.for_ x arr inv var body aim)) out →
+    Exec es (.for_ x arr inv var body aim) out
 
 theorem exec_deterministic {es : ExecState} {s : Stmt} {out1 out2 : Outcome}
     (h1 : Exec es s out1) (h2 : Exec es s out2) : out1 = out2 := by
@@ -300,5 +300,5 @@ theorem exec_deterministic {es : ExecState} {s : Stmt} {out1 out2 : Outcome}
     cases h2 with | execCritical _ _ _ _ hb' => exact ih hb'
   | execThreadEntry _ _ _ hb ih =>
     cases h2 with | execThreadEntry _ _ _ hb' => exact ih hb'
-  | execFor _ _ _ _ _ _ _ hd ih =>
-    cases h2 with | execFor _ _ _ _ _ _ _ hd' => exact ih hd'
+  | execFor _ _ _ _ _ _ _ _ hd ih =>
+    cases h2 with | execFor _ _ _ _ _ _ _ _ hd' => exact ih hd'
